cfrontend/Ctyping.v
@@ -984,6 +984,7 @@ Lemma binarith_type_cast:
   forall t1 t2 m t,
   binarith_type t1 t2 m = OK t -> wt_cast t1 t /\ wt_cast t2 t.
 Proof.
+Local Transparent Ctypes.intsize_eq.
   unfold wt_cast, binarith_type, classify_binarith; intros; DestructCases;
   simpl; split; try congruence;
   try (destruct Archi.ptr64; congruence).
